More effieicnt keygen proof

proof/X-Wing-Correction-Proof.ec
@@ -8,7 +8,7 @@ require import Array4 Array6 Array8 Array32 Array64 Array96 Array140 Array152 Ar
 require import WArray4 WArray6 WArray32 WArray64 WArray96 WArray1088 WArray1120 WArray1184 WArray1216 WArray2400.
 
 axiom shake256_A96_A32 out inp :
-   phoare [Xkem_avx2_clean.M._shake256_A96__A32 :
+  phoare [Xkem_avx2_clean.M._shake256_A96__A32 :
                arg = (out, inp) ==>
                res = SHAKE256_32_96 inp] = 1%r.
 
@@ -18,129 +18,124 @@ axiom sha3_256_A128__A6 ss ss_mlkem ss_x25519 ct_25519 pk_25519 :
                res = SHA3_256_134_32 (ss_mlkem, ss_x25519, ct_25519, pk_25519, xwing_label)] = 1%r.
 
 lemma copy1120 (a : W8.t Array1120.t) :
-Array1120.init (fun (i : int)  =>  WArray1120.get8 (WArray1120.init64
-               (fun (i0 : int) =>  copy_64 (Array140.init
-               (fun (i1 : int) =>  WArray1120.get64 (WArray1120.init8
-               (fun (i2 : int) =>  a.[i2]))  i1)).[i0])) i) = a.
-rewrite tP => k kb.
-rewrite initiE 1:/# /= /get8.
-rewrite initiE 1:/# /= /copy_64.
-rewrite initiE 1:/# /= /get64_direct.
-rewrite W8u8.pack8bE 1:/# /=.
-rewrite initiE 1:/# /=.
-rewrite initiE /#.
+  Array1120.init (fun (i : int)  =>  WArray1120.get8 (WArray1120.init64
+                 (fun (i0 : int) =>  copy_64 (Array140.init
+                 (fun (i1 : int) =>  WArray1120.get64 (WArray1120.init8
+                 (fun (i2 : int) =>  a.[i2]))  i1)).[i0])) i) = a.
+proof.
+  rewrite tP => k kb.
+  rewrite initiE 1:/# /= /get8.
+  rewrite initiE 1:/# /= /copy_64.
+  rewrite initiE 1:/# /= /get64_direct.
+  rewrite W8u8.pack8bE 1:/# /=.
+  rewrite initiE 1:/# /=.
+  rewrite initiE /#.
 qed.
 
 lemma copy1216 (a : W8.t Array1216.t) :
-Array1216.init (fun (i : int)  =>  WArray1216.get8 (WArray1216.init64
-               (fun (i0 : int) =>  copy_64 (Array152.init
-               (fun (i1 : int) =>  WArray1216.get64 (WArray1216.init8
-               (fun (i2 : int) =>  a.[i2]))  i1)).[i0])) i) = a.
-rewrite tP => k kb.
-rewrite initiE 1:/# /= /get8.
-rewrite initiE 1:/# /= /copy_64.
-rewrite initiE 1:/# /= /get64_direct.
-rewrite W8u8.pack8bE 1:/# /=.
-rewrite initiE 1:/# /=.
-rewrite initiE /#.
+  Array1216.init (fun (i : int)  =>  WArray1216.get8 (WArray1216.init64
+                 (fun (i0 : int) =>  copy_64 (Array152.init
+                 (fun (i1 : int) =>  WArray1216.get64 (WArray1216.init8
+                 (fun (i2 : int) =>  a.[i2]))  i1)).[i0])) i) = a.
+proof.
+  rewrite tP => k kb.
+  rewrite initiE 1:/# /= /get8.
+  rewrite initiE 1:/# /= /copy_64.
+  rewrite initiE 1:/# /= /get64_direct.
+  rewrite W8u8.pack8bE 1:/# /=.
+  rewrite initiE 1:/# /=.
+  rewrite initiE /#.
 qed.
 
 
 abbrev toRep4 (x: W8.t Array32.t) = Array4.of_list W64.zero (to_list (unpack64 (pack32 (to_list x)))).
 
 lemma xwing_25519_base_mulx_equiv :
-   equiv [Xkem_avx2_clean.M.xwing_x25519_base ~ Mulx_scalarmult_s.M.__curve25519_mulx_base :
-       _k{2} = toRep4 np{1}
-       ==>
-       res{2} = toRep4 res{1}].
-    proc.
-    inline{1} 4.
-    seq 7 3 : (={u, r, k, _k}). wp. auto => />.
-    move => &1.
-    + rewrite unpack64E pack32E /init8 of_listE.
-    + rewrite tP => i ib.
-    + rewrite initiE 1:/# /= /get8 /(\bits64).
-    + rewrite initiE 1:/# /= /copy_64.
-    + rewrite initiE 1:/# /= /get64_direct.
-    + rewrite /pack8_t. rewrite wordP => ii iib.
-    + rewrite initiE 1:/# //= initiE 1:/# //=.
-    + rewrite initiE 1:/# //= initiE 1:/# //=.
-    + rewrite  initiE 1:/# //= initiE 1:/# //=.
-    + rewrite /to_list /mkseq -iotaredE => />.
-    + smt().
-    seq 4 3 : (={u, k, _k, r} /\ q{1} = r{2}). sim.
-    wp; skip => />.
-    move => &2.
-    + rewrite unpack64E pack32E of_listE.
-    + rewrite tP => i ib.
-    + rewrite initiE 1:/# /= /get8 /(\bits64).
-    + rewrite initiE 1:/# /= /copy_64.
-    + rewrite wordP => ii iib.
-    + rewrite initiE 1:/# /= /init64 /(\bits8).
-    + rewrite initiE 1:/# //= initiE 1:/# //=.
-    + rewrite /to_list /mkseq -iotaredE => />.
-    + smt(W8.initiE).
+  equiv [Xkem_avx2_clean.M.xwing_x25519_base ~ Mulx_scalarmult_s.M.__curve25519_mulx_base :
+    _k{2} = toRep4 np{1}
+    ==>
+    res{2} = toRep4 res{1}].
+proof.
+  proc.
+  inline{1} 4.
+  seq 7 3 : (={u, r, k, _k}). wp. auto => />.
+  move => &1.
+  + rewrite /copy64 tP => i ib.
+  + rewrite unpack64E pack32E /init8 of_listE /get8 /(\bits64).
+  + rewrite !initiE 1,2:/# /=.
+  + rewrite get64E pack8E !initiE 1:/# //=.
+  + rewrite /to_list /mkseq -iotaredE => />.
+  + rewrite wordP => ii iib.
+  rewrite !initiE 1,2:/# //= !initiE 1,2:/# //= !initiE 1,2:/# //= /#.
+
+  seq 4 3 : (={u, k, _k, r} /\ q{1} = r{2}). sim.
+  wp; skip => />.
+  move => &2.
+  + rewrite unpack64E pack32E of_listE.
+  + rewrite tP => i ib.
+  + rewrite initiE 1:/# /= /get8 /(\bits64).
+  + rewrite initiE 1:/# /= /copy_64.
+  + rewrite wordP => ii iib.
+  + rewrite initiE 1:/# /= /init64 /(\bits8).
+  + rewrite initiE 1:/# //= initiE 1:/# //=.
+  + rewrite /to_list /mkseq -iotaredE => />.
+  + smt(W8.initiE).
 qed.
 
 lemma xwing_25519_mulx_equiv :
-   equiv [Xkem_avx2_clean.M.xwing_x25519 ~ Mulx_scalarmult_s.M.__curve25519_mulx :
-       _k{2} = toRep4 np{1}  /\
-       _u{2} = toRep4 pp{1}
-       ==>
-       res{2} = toRep4 res{1}].
-    proc.
-    inline{1} 6.
-    wp; sp.
-    sim :  (={k, u, r}).
-    move => &1 &2 [?] [H] *. rewrite H.
-    + rewrite unpack64E pack32E /init8 of_listE.
-    + rewrite tP => i ib.
-    + rewrite initiE 1:/# /= /get8 /(\bits64).
-    + rewrite initiE 1:/# /= /copy_64.
-    + rewrite /to_list /init64 /(\bits8) /get64_direct /mkseq -iotaredE => />.
-    + rewrite wordP => ii iib.
-    + rewrite initiE 1:/# /=.
-    + rewrite initiE 1:/# //= initiE 1:/# //=.
-    ring. smt(W8.initiE).
-    auto => />. move => &1 *.
-    do split.
-    + rewrite unpack64E pack32E of_listE.
-    + rewrite tP => i ib.
-    + rewrite initiE 1:/# /= /get8 /(\bits64).
-    + rewrite initiE 1:/# /= /copy_64 /get64_direct.
-    + rewrite wordP => ii iib.
-    + rewrite initiE 1:/# /= /init64 /(\bits8) /pack8_t.
-    + rewrite !initiE 1,2:/# //=  initiE 1:/# //= initiE 1:/# //=.
-    + rewrite initiE 1:/# //= initiE 1:/# //=.
-    + rewrite /to_list /mkseq -iotaredE => />. smt().
-    + rewrite unpack64E pack32E of_listE.
-    + rewrite tP => i ib.
-    + rewrite initiE 1:/# /= /get8 /(\bits64).
-    + rewrite initiE 1:/# /= /copy_64 /get64_direct.
-    + rewrite wordP => ii iib.
-    + rewrite initiE 1:/# /= /init64 /(\bits8) /pack8_t.
-    + rewrite !initiE 1,2:/# //=  initiE 1:/# //= initiE 1:/# //=.
-    + rewrite initiE 1:/# //= initiE 1:/# //=.
-    + rewrite /to_list /mkseq -iotaredE => />. smt().
+  equiv [Xkem_avx2_clean.M.xwing_x25519 ~ Mulx_scalarmult_s.M.__curve25519_mulx :
+    _k{2} = toRep4 np{1}  /\
+    _u{2} = toRep4 pp{1}
+    ==>
+    res{2} = toRep4 res{1}].
+proof.
+  proc.
+  inline{1} 6.
+  wp; sp.
+  sim :  (={k, u, r}).
+  move => &1 &2 [?] [H] *. rewrite H.
+  + rewrite unpack64E pack32E /init8 of_listE.
+  + rewrite tP => i ib. rewrite /get8 /(\bits64) /copy_64.
+  + rewrite initiE 1:/# /= initiE 1:/# /=.
+  + rewrite /to_list /init64 /(\bits8) /get64_direct /mkseq -iotaredE => />.
+  + rewrite wordP => ii iib.
+  + rewrite initiE 1:/# /= initiE 1:/# //= initiE 1:/# //=.
+  + ring. smt(W8.initiE).
+  auto => />. move => &1 *.
+  do split.
+  + rewrite unpack64E pack32E of_listE.
+  + rewrite tP => i ib.
+  + rewrite /get8 /(\bits64) /copy_64 /get64_direct /init64 /(\bits8) /pack8_t.
+  + rewrite !initiE 1,2:/# /= !initiE 1:/# /=.
+  + rewrite wordP => ii iib.
+  + rewrite !initiE 1,2:/# /= !initiE 1,2:/# //=  initiE 1:/# //= initiE 1:/# //=.
+  + rewrite /to_list /mkseq -iotaredE => /> /#.
+  + rewrite unpack64E pack32E of_listE.
+  + rewrite tP => i ib.
+  + rewrite /get8 /(\bits64) /copy_64 /get64_direct /init64 /(\bits8) /pack8_t.
+  + rewrite !initiE 1,2:/# /= !initiE 1:/# /=.
+  + rewrite wordP => ii iib.
+  + rewrite !initiE 1,2:/# /= !initiE 1,2:/# //=  initiE 1:/# //= initiE 1:/# //=.
+  + rewrite /to_list /mkseq -iotaredE => /> /#.
 qed.
 
 lemma eq_spec_xwing_25519_base_mulx :
-   equiv [Xkem_avx2_clean.M.xwing_x25519_base ~ CurveProcedures.scalarmult_base :
-      k'{2} =  pack32 (to_list np{1})
-       ==>
-      res{2} = pack32 (to_list res{1})
-   ].
-    transitivity
-    Mulx_scalarmult_s.M.__curve25519_mulx_base
-    (toRep4 np{1} = _k{2} ==> toRep4 res{1} =  res{2})
-    (pack4 (to_list _k{1}) = k'{2} ==> pack4 (to_list res{1}) = res{2}) => />.
-    move => &1.
-    exists(toRep4 np{1}).
-    do split.
-    rewrite of_listK. rewrite size_to_list //=. rewrite to_listK. smt().
-    move => &1. rewrite of_listK. rewrite size_to_list //=. smt().
-    proc *. by call xwing_25519_base_mulx_equiv.
-    proc *. symmetry. by call eq_spec_impl_scalarmult_base_mulx.
+  equiv [Xkem_avx2_clean.M.xwing_x25519_base ~ CurveProcedures.scalarmult_base :
+    k'{2} =  pack32 (to_list np{1})
+    ==>
+    res{2} = pack32 (to_list res{1})].
+proof.
+  transitivity
+  Mulx_scalarmult_s.M.__curve25519_mulx_base
+  (toRep4 np{1} = _k{2} ==> toRep4 res{1} =  res{2})
+  (pack4 (to_list _k{1}) = k'{2} ==> pack4 (to_list res{1}) = res{2}) => />.
+  move => &1.
+  exists(toRep4 np{1}).
+  do split.
+  rewrite of_listK. rewrite size_to_list //=. rewrite to_listK. smt().
+  move => &1. rewrite of_listK. rewrite size_to_list //=. smt().
+  proc *. by call xwing_25519_base_mulx_equiv.
+  proc *. symmetry. by call eq_spec_impl_scalarmult_base_mulx.
 qed.
 
 lemma eq_spec_xwing_25519_mulx :
@@ -148,40 +143,37 @@ lemma eq_spec_xwing_25519_mulx :
        k'{2} = pack32 (to_list np{1}) /\
        u'{2} = pack32 (to_list pp{1})
        ==>
-       res{2} = pack32 (to_list res{1})
-   ].
-    transitivity
-    Mulx_scalarmult_s.M.__curve25519_mulx
-    (toRep4 np{1} = _k{2} /\ toRep4 pp{1} = _u{2}
-     ==> toRep4 res{1} = res{2})
-    (pack4 (to_list _k{1}) = k'{2} /\
-     pack4 (to_list _u{1}) = u'{2}
-     ==> pack4 (to_list res{1}) = res{2}) => />.
-    move => &1 &2 H H0.
-    exists(toRep4 np{1}, toRep4 pp{1}).
-    do split.
-    + rewrite -H. rewrite //= of_listK //=.
-    + rewrite -H0. rewrite //= of_listK //=.
-    move => &1.
-    rewrite of_listK //=  of_listK //=.
-    proc *. by call xwing_25519_mulx_equiv.
-    proc *. symmetry. by call eq_spec_impl_scalarmult_mulx.
+       res{2} = pack32 (to_list res{1})].
+  transitivity
+  Mulx_scalarmult_s.M.__curve25519_mulx
+  (toRep4 np{1} = _k{2} /\ toRep4 pp{1} = _u{2}
+   ==> toRep4 res{1} = res{2})
+  (pack4 (to_list _k{1}) = k'{2} /\
+   pack4 (to_list _u{1}) = u'{2}
+   ==> pack4 (to_list res{1}) = res{2}) => />.
+  move => &1 &2 H H0.
+  exists(toRep4 np{1}, toRep4 pp{1}).
+  do split.
+  + rewrite -H. rewrite //= of_listK //=.
+  + rewrite -H0. rewrite //= of_listK //=.
+  move => &1.
+  rewrite of_listK //=  of_listK //=.
+  proc *. by call xwing_25519_mulx_equiv.
+  proc *. symmetry. by call eq_spec_impl_scalarmult_mulx.
 qed.
 
 lemma eq_spec_xwing_keygen:
   equiv [Xkem_avx2_clean.M._crypto_xkem_keypair_derand_jazz ~ XWing.kg_derand :
-      sk{2} = randomness{1} (** in the rfc, the derand version uses sk to denote the coins **)
-      ==>
-      res{2}.`1 = Array32.init(fun i => res{1}.`2.[i])  /\
-      res{2}.`2.`1.`1 = Array1152.init(fun i => res{1}.`1.[i]) /\
-      res{2}.`2.`1.`2 = Array32.init(fun i => res{1}.`1.[i+1152]) /\
-      res{2}.`2.`2 = Array32.init(fun i => res{1}.`1.[i+1184])].
+    sk{2} = randomness{1} (** in the rfc, the derand version uses sk to denote the coins **)
+    ==>
+    res{2}.`1 = Array32.init(fun i => res{1}.`2.[i])  /\
+    res{2}.`2.`1.`1 = Array1152.init(fun i => res{1}.`1.[i]) /\
+    res{2}.`2.`1.`2 = Array32.init(fun i => res{1}.`1.[i+1152]) /\
+    res{2}.`2.`2 = Array32.init(fun i => res{1}.`1.[i+1184])].
 proof.
   proc => />.
   proc rewrite {1} 8 (copy32). inline {2} 1. auto => />.
-  seq 9 2 : (#pre /\ expanded{1} = SHAKE256_32_96 randomness{1}
-                  /\ randomness{1} = srandomness{1}
-                  /\ ={expanded}
+  seq 9 2 : (#pre /\ ={expanded}
                   /\ srandomness{1} = sk0{2}
                   /\ srandomness{1} = sk{2}).
   + ecall {1} (shake256_A96_A32 expanded{1} srandomness{1}); wp; skip => />.
@@ -198,39 +190,28 @@ proof.
                   /\ coins2{2} = Array32.init (fun (i : int ) => expanded{1}.[32 + i])
                   /\ coins1{2} = Array32.init (fun (i : int ) => expanded{2}.[i])
                   /\ coins2{2} = Array32.init (fun (i : int ) => expanded{2}.[32+i])).
-  + auto => />. move => &1. do split.  rewrite tP => i ib. rewrite !initiE 1..5:/# //=.
-  + rewrite tP => i ib. rewrite !initiE 1..2:/# //= !initiE 1..3:/# //=.
+  + auto => />. move => &1. do split.  rewrite tP => i ib. rewrite !initiE 1..3:/# //=.
+  + rewrite tP => i ib. rewrite !initiE 1..2:/# //= !initiE 1..2:/# //=.
 
   auto => />.
   seq 0 1 : (#pre /\ expanded_x25519{1} = sk_X0{2}
-                  /\ sk_X0{2} = coins3{2}).
-  + auto => />.
+                  /\ sk_X0{2} = coins3{2}). auto => />.
 
   seq 1 1 : (#pre /\ pack32 (to_list pk_x25519{1}) = pk_X_256{2}).
   + call eq_spec_xwing_25519_base_mulx. auto => />.
 
-  seq 0 1 : (#pre /\ pk_x25519{1} = pk_X0{2}
-                  /\ pk_x25519{1} = Array32.of_list W8.zero (W32u8.to_list pk_X_256{2})). auto => />.
-  + move => &1 &2 [#] *. rewrite !tP. do split.
-  + move => i ib. rewrite !/to_list !/mkseq -!iotaredE => />. rewrite !/of_list initiE 1:/# //=. smt().
-  + move => i ib. rewrite !/to_list !/mkseq -!iotaredE => />. rewrite !/of_list initiE 1:/# //=. smt().
+  seq 0 1 : (#pre /\ pk_x25519{1} = pk_X0{2}). auto => />.
+  + move => &1 &2 [#] *. rewrite !tP.
+  + move => i ib. rewrite !/to_list !/mkseq -!iotaredE => />. rewrite !/of_list initiE 1:/# //= /#.
 
-  seq 1 1 : (#pre /\ pk_M0{2}.`1 = (init (fun (i : int) =>  pk_mlkem{1}.[i]))%Array1152
-                  /\ pk_M0{2}.`2 = (init (fun (i : int) =>  pk_mlkem{1}.[i + 1152]))%Array32
-                  /\ let (t,rho) = pk_M0{2} in
-                     sk_M0{2}.`1 = Array1152.init(fun i => sk_mlkem{1}.[i])
+  seq 1 1 : (#pre /\ pk_M0{2}.`1 = Array1152.init (fun (i : int) =>  pk_mlkem{1}.[i])
+                  /\ pk_M0{2}.`2 = Array32.init(fun (i : int) =>  pk_mlkem{1}.[i + 1152])
+                  /\ sk_M0{2}.`1 = Array1152.init(fun i => sk_mlkem{1}.[i])
                   /\ sk_M0{2}.`2.`1 = Array1152.init(fun i => sk_mlkem{1}.[i+1152])
                   /\ sk_M0{2}.`2.`2 = Array32.init(fun i => sk_mlkem{1}.[i+1152+1152])
                   /\ sk_M0{2}.`3 = Array32.init(fun i => sk_mlkem{1}.[i+1152+1152 + 32])
-                  /\ sk_M0{2}.`4 = Array32.init(fun i => sk_mlkem{1}.[i+1152+1152 + 32 + 32])
-                  /\ t = Array1152.init(fun i => pk_mlkem{1}.[i])
-                  /\ rho = Array32.init(fun i => pk_mlkem{1}.[i+1152])).
+                  /\ sk_M0{2}.`4 = Array32.init(fun i => sk_mlkem{1}.[i+1152+1152 + 32 + 32])).
   + call mlkem_kem_correct_kg. auto => />. smt(). auto => />.
-
-  seq 9 0 : (#pre /\ sk0{2} = (init ("_.[_]" skp{1}))%Array32
-                  /\ pk_M0{2}.`1 = (init ("_.[_]" pkp{1}))%Array1152
-                  /\ pk_M0{2}.`2 = (init (fun (i0 : int) => pkp{1}.[i0 + 1152]))%Array32
-                  /\ pk_X0{2} = (init (fun (i0 : int) => pkp{1}.[i0 + 1184]))%Array32).
 
   seq 3 0 : (#pre /\ pk_M0{2}.`1 = (init (fun (i : int) =>  pk_mlkem{1}.[i]))%Array1152
                   /\ pk_M0{2}.`2 = (init (fun (i : int) =>  pk_mlkem{1}.[i + 1152]))%Array32
@@ -246,36 +227,38 @@ proof.
                    /\ (forall k, 0<=k<min (8 * i{1}) 1152 => pkp{1}.[k] = pk_M0{2}.`1.[k])
                    /\ (forall k, 1152<=k<min (8 * i{1}) 1184 => pkp{1}.[k] = pk_M0{2}.`2.[k-1152]))
               (148 - i{1}).
-   + auto => />. move => &hr Z. rewrite !tP. move => H H0 H1 H2 H3 H4 H5 H6 H7 H8 H9. do split.
-   + smt(). smt(). move => i ib *. rewrite !initE.
+   + auto => />. move => &hr Z. rewrite !tP. move => H H0 H1 H2 H3 H4 H5 H6 H7 H8 H9 H10 H11 H12.
+   + do split; 1,2:smt().
+   + move => i ib *. rewrite !initE.
    + case(0 <= i && i < 1184) => *. rewrite ifT 1:/#.
    + rewrite get8_set64_directE 1,2:/#. case (8 * i{!hr} <= i && i < 8 * i{!hr} + 8) => *.
    + rewrite get64E /get8 /init8 !pack8bE 1:/# !initiE 1:/# //= !initiE 1:/# /#.
    + rewrite /get8 /init8 !initiE 1:/#. smt(). smt().
    + move => i ib *.
-   + case(0 <= i && i < 1152) => *. rewrite H1. smt().
-   + rewrite !initiE 1,2:/#.
+   + case(0 <= i && i < 1152) => *.
+   + rewrite !initiE 1:/#.
    + rewrite get8_set64_directE 1,2:/#. case (8 * i{!hr} <= i && i < 8 * i{!hr} + 8) => *.
-   + rewrite get64E /get8 /init8 !pack8bE 1:/# !initiE 1:/# //= !initiE 1:/# /#.
-   + rewrite /get8 /init8 !initiE 1:/#. smt(). rewrite !initiE 1,2:/#.
+   + rewrite get64E /get8 /init8 !pack8bE 1:/# !initiE 1:/# //= !initiE 1:/# H0 1:/#.
+   + rewrite /get8 /init8 !initiE 1:/# /#.
+   + rewrite /get8 /init8 !initiE 1:/# /#.
+   + rewrite /get8 /init8 !initiE 1:/# /#.
    + move => i ib *.
    + rewrite !initiE 1:/#.
    + rewrite get8_set64_directE 1,2:/#. case (8 * i{!hr} <= i && i < 8 * i{!hr} + 8) => *.
-   + rewrite get64E /get8 /init8 !pack8bE 1:/# !initiE 1:/# //= !initiE 1:/# H2 1:/# !initiE 1:/# //= /#.
-   + rewrite /get8 /init8 !initiE 1:/#. smt(). smt().
+   + rewrite get64E /get8 /init8 !pack8bE 1:/# !initiE 1:/# //= !initiE 1:/# H1 1:/# !initiE 1:/# //= /#.
+   + rewrite /get8 /init8 !initiE 1:/# /#. smt().
 
    + wp. auto => />.
-   + move => &1 &2 [#] H H0 H1 H2 H3 H4. auto => />. do split.
-   + smt(). smt(). smt(). move => ??. do split.
-   + move => H5 H6 H7 H8 H9 H10. smt(). move => H11 H12 H13 H14 H15 H16. rewrite tP. do split.
+   + move => &1 &2 [#] H H0 H1 H2 H3 H4 H5 H6 H7. auto => />. do split;1..3:smt().
+   + move => ??. do split.
+   + move => H8 H9 H10 H11 H12 /#. move => H11 H12 H13 H14 H15 H16. rewrite tP. do split.
    + move => H17 H18. rewrite -H15 1:/#. smt(Array1152.initiE).
-   + rewrite H3. rewrite tP => i ib. rewrite !initiE 1,2:/# //= -H14 1,2:/#.
+   + rewrite H2  tP => i ib. rewrite !initiE 1,2:/# //= -H14 1,2:/#.
 
-   seq 3 0 : (#pre /\ pk_X0{2} = (init (fun (i0 : int) => pkp{1}.[i0 + 1184]))%Array32
-                   /\ pk_x25519{1} = (init (fun (i0 : int) => pkp{1}.[i0 + 1184]))%Array32
-                   /\ pk_X0{2} = pk_x25519{1}).
-   wp.
-   while{1} (#pre /\ aux{1} = 4
+   seq 3 0 : (#pre /\ pk_X0{2} = Array32.init (fun (i0 : int) => pkp{1}.[i0 + 1184])
+                   /\ pk_x25519{1} = Array32.init (fun (i0 : int) => pkp{1}.[i0 + 1184])).
+   + wp.
+   + while{1} (#pre /\ aux{1} = 4
                   /\ 0 <= i{1} <= aux{1}
                   /\ pk_X0{2} = pk_x25519{1}
                   /\ (forall k, 0<=k<min (8 * i{1}) 32 => pkp{1}.[k+1184] = pk_x25519{1}.[k])
@@ -283,65 +266,66 @@ proof.
                   /\ (forall k, 1184<=k<min (8 * i{1}) 1216 => pkp{1}.[k] = pk_x25519{1}.[k-1216])
                   /\ (forall k, 1184<=k<min (8 * i{1}) 1216 => pkp{1}.[k] = pk_X0{2}.[k-1216]))
               (4 - i{1}).
-
-   + auto => />. move => &hr Z. rewrite !tP. move => H H0 H1 H2 H3 H4 H5 H6 H7 H8 H9 H10. do split.
+   + auto => />. move => &hr Z. rewrite !tP.
+   move => [#] H H0 H1 H2 H3 H4 H5 H6 H7 H8 H9 H10 H11 H12 H13. do split.
    + move => i ib. rewrite !initiE 1,2:/# /=.
    + rewrite get8_set64_directE 1,2:/# ifF 1:/#.
-   + rewrite /get8 /init8 !initiE 1:/# H4 1:/#. smt(Array1152.initiE).
+   + rewrite /get8 /init8 !initiE 1:/# H7 1:/#. smt(Array1152.initiE).
    + move => i ib. rewrite !initiE 1:/# /= !initiE 1:/#.
    + rewrite get8_set64_directE 1,2:/# ifF 1:/#.
-   + rewrite /get8 /init8 !initiE 1:/# H5 1:/#. smt(Array32.initiE).
-   smt(). smt().
+   + rewrite /get8 /init8 !initiE 1:/# H8 1:/#. smt(Array32.initiE).
+   + smt(). smt().
    + move => k0 i ib. rewrite !initiE 1:/# /=.
    + rewrite get8_set64_directE 1,2:/#.
    + case (8 * (148 + i{!hr}) <= k0 + 1184 && k0 + 1184 < 8 * (148 + i{!hr}) + 8) => *.
    + rewrite get64E /get8 /init8 !pack8bE 1:/# !initiE 1:/# //= !initiE 1:/# /# //=.
-   + rewrite /get8 /init8 !initiE 1:/# H8 1:/# /#.
+   + rewrite /get8 /init8 !initiE 1:/# H11 1:/# /#.
    + move => k0 i ib. rewrite !initiE 1:/# /=.
    + rewrite get8_set64_directE 1,2:/#.
    + case (8 * (148 + i{!hr}) <= k0 + 1184 && k0 + 1184 < 8 * (148 + i{!hr}) + 8) => *.
    + rewrite get64E /get8 /init8 !pack8bE 1:/# !initiE 1:/# //= !initiE 1:/# /# //=.
-   + rewrite /get8 /init8 !initiE 1:/# H8 1:/# /#.
+   + rewrite /get8 /init8 !initiE 1:/# H11 1:/# /#.
    + move => k0 i ib. rewrite !initiE 1:/# /=.
    + rewrite get8_set64_directE 1,2:/#. rewrite ifF 1:/#.
-   + rewrite /get8 /init8 !initiE 1:/# H9 1:/# /#.
+   + rewrite /get8 /init8 !initiE 1:/# H12 1:/# /#.
    + move => k0 i ib. rewrite !initiE 1:/# /=.
    + rewrite get8_set64_directE 1,2:/#. rewrite ifF 1:/#.
-   + rewrite /get8 /init8 !initiE 1:/# H9 1:/# /#. smt().
+   + rewrite /get8 /init8 !initiE 1:/# H12 1:/# /#. smt().
 
-   + wp. auto => />. rewrite !tP. move => &1 &2 [#] H H0 H1 H2 H3 H4 H5 H6. do split.
-   + smt(). smt(). smt(). smt().
-   + move => H7 H8. do split. move => H9 H10 H11 H12 H13 H14. smt().
+   + wp. auto => />. rewrite !tP. move => &1 &2 [#] H H0 H1 H2 H3 H4 H5 H6 H7 H8 H9.
+   + do split;1..4:smt().
+   + move => H10 H11. do split. move => H12 H13 H14 H15 H16 H17 H18. smt().
    + move => H15 H16 H17 H18 H19 H20 H21. rewrite tP. do split.
    + move => i ib. rewrite !initiE 1:/# //=. smt().
    + move => i ib. rewrite !initiE 1:/# //=. smt().
 
-   seq 3 0 : (#pre /\ sk{2} = skp{1} /\ sk0{2} = skp{1} /\ skp{1} = srandomness{1}).
-   while{1} (#pre /\ aux{1} = 4
+   seq 3 0 : (#pre /\ sk{2} = skp{1}).
+   + while{1} (#pre /\ aux{1} = 4
                   /\ 0 <= i{1} <= aux{1}
                   /\ sk{2} = srandomness{1}
                   /\ sk0{2} = srandomness{1}
                   /\ (forall k, 0<=k<min (8 * i{1}) 32 => skp{1}.[k] = sk{2}.[k])
                   /\ (forall k, 0<=k<min (8 * i{1}) 32 => skp{1}.[k] = sk0{2}.[k]))
               (4 - i{1}).
-   + auto => />. move => &hr Z. rewrite !tP. move => H H0 H1 H2 H3 H4 H5 H6 H7 H8 H9. do split.
-   + smt(). smt(). move => i ib *. rewrite !initiE 1:/#.
-   + rewrite get8_set64_directE 1,2:/#. case(8 * i{!hr} <= i && i < 8 * i{!hr} + 8) => *.
-   + rewrite get64E /get8 /init8 !pack8bE 1:/# !initiE 1:/# //= !initiE 1:/# /# //=.
-   + rewrite /get8 /init8 !initiE 1:/# H8 1:/# /#.
+   + auto => />. move => &hr Z. rewrite !tP. move => H H0 H1 H2 H3 H4 H5 H6 H7 H8 H9 H10 H11 H12.
+   + do split; 1,2:smt().
    + move => i ib *. rewrite !initiE 1:/#.
    + rewrite get8_set64_directE 1,2:/#. case(8 * i{!hr} <= i && i < 8 * i{!hr} + 8) => *.
    + rewrite get64E /get8 /init8 !pack8bE 1:/# !initiE 1:/# //= !initiE 1:/# /# //=.
-   + rewrite /get8 /init8 !initiE 1:/# H8 1:/# /#. smt().
-   wp. auto => />.
-   move => &1 &2 [#] *. do split. smt(). smt(). move => I I0. do split.
-   smt(). move => [#] H H0 H1 H2. do split.
-   rewrite tP => i ib. rewrite H2. smt(). smt().
-   rewrite tP => i ib. rewrite H2. smt(). smt().
-   rewrite tP => i ib. rewrite H2. smt(). smt().
+   + rewrite /get8 /init8 !initiE 1:/# H11 1:/# /#.
+   + move => i ib *. rewrite !initiE 1:/#.
+   + rewrite get8_set64_directE 1,2:/#. case(8 * i{!hr} <= i && i < 8 * i{!hr} + 8) => *.
+   + rewrite get64E /get8 /init8 !pack8bE 1:/# !initiE 1:/# //= !initiE 1:/# /# //=.
+   + rewrite /get8 /init8 !initiE 1:/# H11 1:/# /#. smt().
+
+   + wp. auto => />.
+   + move => &1 &2 [#] *. do split. smt(). smt(). move => I I0. do split.
+   + smt(). move => [#] H H0 H1 H2.
+   + rewrite tP => i ib. rewrite H2 1,2:/#.
+
    wp. auto => />. rewrite !tP.
-   move => &1 &2 H H0 H1 H2 H3 H4 H5 H6. move => i ib. rewrite initiE 1,2:/#.
-   wp. auto => />.
+   move => &1 &2 H H0 H1 H2 H3 H4 H5 H6 H7 H8 H9 H10 H11.
+   rewrite initiE 1,2:/#.
 qed.
 
 
@@ -386,6 +370,7 @@ proof.
     seq 1 1  : (#pre /\ c_M{2} = seed_mlkem{1}
                      /\ c_M{2} = Array32.init (fun (i:int) => seseed{1}.[i])).
     + auto => />.
+
     seq 1 1 : (#pre /\ pack32 (to_list ct_x25519{1}) = ct_X_256{2}).
     + call eq_spec_xwing_25519_base_mulx. auto => />.
     + move => &1 &2 H H0 H1 H2 H3 H4 H5 H6 H7 H8 H9.
@@ -399,13 +384,13 @@ proof.
 
     seq 0 1 : (#pre /\ ct_X{2} = ct_x25519{1}).
     + auto => />. move => &1 &2 H H0 H1 H2 H3 H4 H5 H6 H7 H8 H9.
-    rewrite !/of_list !/to_list !/mkseq -iotaredE => />.
-    rewrite tP => i ib. rewrite initiE 1,2:/#.
+    + rewrite !/of_list !/to_list !/mkseq -iotaredE => />.
+    + rewrite tP => i ib. rewrite initiE 1,2:/#.
 
     seq 0 1 : (#pre /\ ss_X{2} = ss_x25519{1}).
     + auto => />. move => &1 &2 H H0 H1 H2 H3 H4 H5 H6 H7 H8 H9.
-    rewrite !/of_list !/to_list !/mkseq -iotaredE => />.
-    rewrite tP => i ib. rewrite initiE 1,2:/#.
+    + rewrite !/of_list !/to_list !/mkseq -iotaredE => />.
+    + rewrite tP => i ib. rewrite initiE 1,2:/#.
 
    seq 2 3 : (#pre /\ ct_M{2}.`1 = Array960.init(fun i => ct_mlkem{1}.[i])
                    /\ ct_M{2}.`2 = Array128.init(fun i => ct_mlkem{1}.[i+960])
@@ -426,7 +411,6 @@ proof.
     + congr. congr. smt(). + rewrite tP => i ib. smt(Array32.initiE).
 
     wp. auto => />.
-    auto => />.
     + seq 3 0 : (#pre  /\ ct{2}.`1.`1 = Array960.init(fun i => ctp{1}.[i])
                        /\ ct{2}.`1.`2 = Array128.init(fun i => ctp{1}.[i+960])
                        /\ ct{2}.`1.`1 = Array960.init(fun i => ct_mlkem{1}.[i])
@@ -436,7 +420,6 @@ proof.
                        /\ ct_M{2}.`1 = ct{2}.`1.`1
                        /\ ct_M{2}.`2 = ct{2}.`1.`2
                        /\ ct_X{2} = ct{2}.`2).
-
     + while{1} (#pre /\ aux{1} = 136
                      /\ ct{2}.`1.`1 = Array960.init(fun i => ct_mlkem{1}.[i])
                      /\ ct{2}.`1.`2 = Array128.init(fun i => ct_mlkem{1}.[i+960])
@@ -481,11 +464,11 @@ proof.
     + rewrite get64E /init8 pack8bE 1:/# !initiE 1:/# //= !initiE 1:/# //= /#.
     + rewrite /get8 /init8. rewrite -H17 1:/# !initiE 1:/# //=. smt().
 
-    wp. auto => />. move => &1 &2 H H0 H1 H2 H3 H4 H5 H6 H7 H8 H9 H10 H11 H12 H13 H14 H15 H16.
-    do split;1..6:smt().
-    move => H17 H18. do split. move => *. smt(). move => *. do split. rewrite tP => i ib.
-    rewrite initiE 1:/#. smt(). rewrite tP => i ib. rewrite initiE 1:/#. smt(). rewrite tP => i ib.
-    rewrite initiE 1:/#. smt(). rewrite tP => i ib. rewrite initiE 1:/#. smt().
+    + wp. auto => />. move => &1 &2 H H0 H1 H2 H3 H4 H5 H6 H7 H8 H9 H10 H11 H12 H13 H14 H15 H16.
+    + do split;1..6:smt().
+    + move => H17 H18. do split. move => *. smt(). move => *. do split. rewrite tP => i ib.
+    + rewrite initiE 1:/#. smt(). rewrite tP => i ib. rewrite initiE 1:/#. smt(). rewrite tP => i ib.
+    + rewrite initiE 1:/#. smt(). rewrite tP => i ib. rewrite initiE 1:/#. smt().
 
     wp. auto => />.
     + seq 3 0 : (#pre /\ ct_X{2} = Array32.init(fun i => ctp{1}.[i+1088])
@@ -498,7 +481,7 @@ proof.
     + auto => />. move => &hr Z. rewrite !tP.
     + move => H H0 H1 H2 H3 H4 H5 H6 H7 H8 H9 H10 H11 H12.
     + move => H13 H14 H15 H16 H17 H18 H19 H20 H21 H22 H23.
-    do split.
+    + do split.
     + move => i b *. rewrite H16 1:/# !initiE 1..3:/#.
     + rewrite get8_set64_directE 1,2:/# ifF 1:/#.
     + rewrite /get8 /init8 !initiE 1,2:/# /=.
@@ -518,11 +501,11 @@ proof.
     + rewrite get64E /init8 pack8bE 1:/# !initiE 1:/# //= !initiE 1:/# //= /#.
     + rewrite /get8 /init8. rewrite -H22 1:/# !initiE 1,2:/# //= /#. smt().
 
-    wp. simplify. skip => />.
-    move => &1 &2 [#] H H0 H1 H2 H3 H4 H5 H6 H7 H8 H9 H10 H11 H12 H13 H14 H15 H16 H17 H18 H19 H20.
-    do split. smt(). move => [#] H21 H22. do split. move => [#] H23 H24 H25 H26 H27 H28 H29 H30.
-    smt(). move => [#] H31 H32 H33 H34 H35 H36 H37 H38. do split. rewrite tP => i ib.
-    rewrite !initiE 1:/# //=. smt(). rewrite tP => i ib. rewrite !initiE 1:/# //=. smt().
+    + wp. simplify. skip => />.
+    + move => &1 &2 [#] H H0 H1 H2 H3 H4 H5 H6 H7 H8 H9 H10 H11 H12 H13 H14 H15 H16 H17 H18 H19 H20.
+    + do split. smt(). move => [#] H21 H22. do split. move => [#] H23 H24 H25 H26 H27 H28 H29 H30.
+    + smt(). move => [#] H31 H32 H33 H34 H35 H36 H37 H38. do split. rewrite tP => i ib.
+    + rewrite !initiE 1:/# //=. smt(). rewrite tP => i ib. rewrite !initiE 1:/# //=. smt().
 
     wp. auto => />.
     + seq 3 0 : (#pre  /\ ss{2} = shkp{1} /\ ={ss} /\ shkp{1} = ss{1}).
@@ -543,11 +526,11 @@ proof.
     + move => i ib *.  rewrite !initiE 1:/#.
     + rewrite get8_set64_directE 1,2:/#. case(8 * i{!hr} <= i && i < 8 * i{!hr} + 8) => *.
     + rewrite get64E /init8 pack8bE 1:/# !initiE 1:/# //= !initiE 1:/# //= /#.
-    + rewrite /get8 /init8 -H23 1:/#. smt(WArray32.initiE).  smt().
-    wp. simplify. skip => />.
-    move => &1 &2 [#] H H0 H1 H2 H3 H4 H5 H6 H7 H8 H9 H10 H11 H12 H13 H14 H15 H16 H17 H18 H19 H20 H21.
-    do split. smt(). move => [#] H22 H23 H24. smt(). move => [#] H24 H25. do split. smt().
-    move => [#] H28 H29 H30 H31. do split. rewrite tP => i ib. smt(). rewrite tP => i ib. smt().
+    + rewrite /get8 /init8 -H23 1:/#. smt(WArray32.initiE). smt().
+    + wp. simplify. skip => />.
+    + move => &1 &2 [#] H H0 H1 H2 H3 H4 H5 H6 H7 H8 H9 H10 H11 H12 H13 H14 H15 H16 H17 H18 H19 H20 H21.
+    + do split. smt(). move => [#] H22 H23 H24. smt(). move => [#] H24 H25. do split. smt().
+    + move => [#] H28 H29 H30 H31. do split. rewrite tP => i ib. smt(). rewrite tP => i ib. smt().
     auto => />.
 qed.
 
@@ -590,8 +573,7 @@ proof.
 
   auto => />.
   seq 0 1 : (#pre /\ expanded_x25519{1} = sk_X0{2}
-                  /\ sk_X0{2} = coins3{2}).
-  + auto => />.
+                  /\ sk_X0{2} = coins3{2}). auto => />.
   swap{1} 1 1.
   seq 1 1 : (#pre /\ pack32 (to_list pk_x25519{1}) = pk_X_256{2}).
   + call eq_spec_xwing_25519_base_mulx. auto => />.
@@ -653,7 +635,7 @@ proof.
   + ecall {1} (sha3_256_A128__A6 ss{1} ss_mlkem{1} ss_x25519{1} ct_x25519{1} pk_x25519{1}).
   + wp; skip => />.
 
-  + seq 3 0 : (#pre  /\ ss{2} = shkp{1} /\ ={ss} /\ shkp{1} = ss{1}).
+  seq 3 0 : (#pre  /\ ss{2} = shkp{1} /\ ={ss} /\ shkp{1} = ss{1}).
 
     + while{1} (#pre /\ aux{1} = 4
                      /\ 0 <= i{1} <= 4
@@ -672,10 +654,10 @@ proof.
     + rewrite get8_set64_directE 1,2:/#. case(8 * i{!hr} <= i && i < 8 * i{!hr} + 8) => *.
     + rewrite get64E /init8 pack8bE 1:/# !initiE 1:/# //= !initiE 1:/# //= /#.
     + rewrite /get8 /init8 -H18 1:/#. smt(WArray32.initiE).  smt().
-    wp. simplify. skip => />.
-    move => &1 &2 [#] H H0 H1 H2 H3 H4 H5 H6 H7 H8 H9 H10 H11 H12 H13 H14 H15 H16.
-    do split. smt(). move => [#] H22 H23 H24. smt(). move => [#] H24 H25. do split. smt().
-    move => [#] H28 H29 H30 H31. do split. rewrite tP => i ib. smt(). rewrite tP => i ib. smt().
+    + wp. simplify. skip => />.
+    + move => &1 &2 [#] H H0 H1 H2 H3 H4 H5 H6 H7 H8 H9 H10 H11 H12 H13 H14 H15 H16.
+    + do split. smt(). move => [#] H22 H23 H24. smt(). move => [#] H24 H25. do split. smt().
+    + move => [#] H28 H29 H30 H31. do split. rewrite tP => i ib. smt(). rewrite tP => i ib. smt().
     auto => />.
 qed.
 
